src/Common/List/Prefix.v
@@ -1,0 +1,33 @@
+(* Prefix of a list.*)
+Require Import Coq.Lists.List ADTSynthesis.Common.
+Section Prefix.
+
+  Context {A : Type}.
+  Context {A_eq_dec : forall (a a' : A), {a = a'} + {a <> a'}}.
+
+  Definition prefixProp (p s : list A) := exists ps, p ++ ps = s.
+
+  Fixpoint prefixBool (p s : list A) :=
+    match p, s with
+      | nil , _ => true
+      | p' :: ps', s' :: ss' => if A_eq_dec p' s' then prefixBool ps' ss' else false
+      | _, _ => false
+    end.
+
+  Lemma prefixBool_eq :
+    forall (p s : list A),
+      prefixBool p s = true <-> prefixProp p s.
+  Proof.
+    unfold prefixProp; split; revert s; induction p; intros s H.
+    - eexists s; reflexivity.
+    - destruct s; simpl in H.
+      + discriminate.
+      + find_if_inside; [subst | discriminate].
+        apply_in_hyp IHp; destruct_ex; eexists; subst; reflexivity.
+    - simpl; reflexivity.
+    - destruct s; simpl in *; destruct H.
+      + discriminate.
+      + injections; find_if_inside; intuition eauto.
+  Qed.
+
+End Prefix.
