src/Common/List/UpperBound.v
@@ -1,0 +1,58 @@
+(* UpperBound of a list.*)
+Require Import Coq.Lists.List ADTSynthesis.Common.
+Section UpperBound.
+
+  Context {A : Type}.
+  Variable R : A -> A -> Prop.
+  Context {Pre_R : PreOrder R}.
+
+  Definition upperbound (As : list A) (r : A) :=
+    forall r', In r' As -> R r' r.
+
+  Variable (R_dec : forall a a', {R a a'} + {R a' a}).
+  Context {MinA : A}.
+  Variable R_MinA : forall a : A, R MinA a.
+
+  Definition find_max
+             (As : list A) : A := 
+    fold_right (fun a acc => if R_dec a acc then acc else a) MinA As.
+
+  Lemma fold_right_max_is_max
+  : forall As a,
+      In a As -> R a (find_max As).
+  Proof.
+    induction As; intros; inversion H; subst; simpl;
+    find_if_inside; intros; eauto.
+    - reflexivity.
+    - etransitivity; eauto.
+  Qed.
+  
+  Definition find_upperbound
+             (As : list A) : list A :=
+    let max := find_max As in
+    filter (fun a => if R_dec max a then true else false) As.
+
+  Lemma fold_right_higher_is_higher
+  : forall As a,
+      (forall a', In a' As -> R a' a) ->
+      R (find_max As) a.
+  Proof.
+    induction As; simpl; intros; [ apply R_MinA | ].
+    find_if_inside;
+    etransitivity; eauto; reflexivity.
+  Qed.
+
+  Lemma find_upperbound_highest_length
+  : forall As a,
+      In a (find_upperbound As) -> forall a', In a' As -> R a' a.
+  Proof.
+    unfold find_upperbound; intros.
+    apply filter_In in H; intuition.
+    destruct (R_dec (find_max As) a).
+    etransitivity.
+    eapply fold_right_max_is_max; eauto.
+    eassumption.
+    discriminate.
+  Qed.
+
+End UpperBound.
